rupicola/stlc_v2/TypRel.fst
@@ -30,6 +30,13 @@ let test_match s (r:rtyp s) = (** why does this work so well? **)
   | RArr #s1 #s2 _ _ -> assert (s == (s1 -> s2))
   | RPair #s1 #s2 _ _ -> assert (s == (s1 & s2))
 
+let rec rtype_to_ttype s (r:rtyp s) : typ =
+  match r with
+  | RUnit -> TUnit
+  | RBool -> TBool
+  | RArr #s1 #s2 rs1 rs2 -> TArr (rtype_to_ttype s1 rs1) (rtype_to_ttype s2 rs2)
+  | RPair #s1 #s2 rs1 rs2 -> TPair (rtype_to_ttype s1 rs1) (rtype_to_ttype s2 rs2)
+
 type typsr =
   s:Type & rtyp s
 
@@ -107,3 +114,59 @@ let lem_gsubst_closed_identiy #g #b (s:gsub g b) (e:closed_exp) :
   Lemma (gsubst s e == e)
   [SMTPat (gsubst s e)] =
   admit ()
+
+noeq type typing : env -> exp -> typ -> Type =
+  | TyUnit : #g:env ->
+             typing g EUnit TUnit
+  | TyTrue : #g:env ->
+             typing g ETrue TBool
+  | TyFalse : #g:env ->
+              typing g EFalse TBool
+  | TyIf : #g:env ->
+           #e1:exp ->
+           #e2:exp ->
+           #e3:exp ->
+           #t:typ ->
+           $h1:typing g e1 TBool ->
+           $h2:typing g e2 t ->
+           $h3:typing g e3 t ->
+             typing g (EIf e1 e2 e3) t
+  //| TyVar : #g:env ->
+  //          x:var{Some? (g x)} ->
+  //            typing g (EVar x) (rtype_to_ttype (get_Type (Some?.v (g x))) (get_rel (Some?.v (g x))))
+  //| TyLam : #g:env ->
+  //          #body:exp ->
+  //          #t1:typ ->
+  //          #t2:typ ->
+  //          $hbody:typing (extend t1 g) body t2 ->
+  //            typing g (ELam body) (TArr t1 t2)
+  | TyApp : #g:env ->
+            #e1:exp ->
+            #e2:exp ->
+            #t1:typ ->
+            #t2:typ ->
+            $h1:typing g e1 (TArr t1 t2) -> 
+            $h2:typing g e2 t1 ->
+              typing g (EApp e1 e2) t2
+   | TyPair : #g:env ->
+             #e1:exp ->
+             #e2:exp ->
+             #t1:typ ->
+             #t2:typ ->
+             $h1:typing g e1 t1 ->
+             $h2:typing g e2 t2 ->
+               typing g (EPair e1 e2) (TPair t1 t2)
+  | TyFst : #g:env ->
+            #e:exp ->
+            #t1:typ ->
+            #t2:typ ->
+            $h1:typing g e (TPair t1 t2) ->
+              typing g (EFst e) t1
+  | TySnd : #g:env ->
+            #e:exp ->
+            #t1:typ ->
+            #t2:typ ->
+            $h1:typing g e (TPair t1 t2) ->
+              typing g (ESnd e) t2
+             
+  
